src/cbor/CBOR.Spec.Raw.Sort.fsti
@@ -69,8 +69,69 @@ let cbor_raw_sort_elem_equiv
 = raw_equiv_eq x (cbor_raw_sort_elem x);
   match x with
   | Map len v ->
-    list_for_all_intro (list_existsb2 (holds_on_pair2 raw_equiv) (cbor_map_sort_failsafe v)) v (fun _ -> assume False);
-    list_for_all_intro (list_existsb2 (holds_on_pair2 raw_equiv) v) (cbor_map_sort_failsafe v) (fun _ -> assume False)    
+    list_for_all_intro (list_existsb2 (holds_on_pair2 raw_equiv) (cbor_map_sort_failsafe v)) v (fun x ->
+      raw_equiv_refl (fst x);
+      raw_equiv_refl (snd x);
+      list_existsb_intro (holds_on_pair2 raw_equiv x) (cbor_map_sort_failsafe v) x
+    );
+    list_for_all_intro (list_existsb2 (holds_on_pair2 raw_equiv) v) (cbor_map_sort_failsafe v) (fun x ->
+      raw_equiv_refl (fst x);
+      raw_equiv_refl (snd x);
+      list_existsb_intro (holds_on_pair2 raw_equiv x) v x
+    )
   | _ -> raw_equiv_refl x
 
 let cbor_raw_sort = raw_data_item_fmap cbor_raw_sort_elem
+
+let rec cbor_raw_sort_ints_optimal
+  (x: raw_data_item)
+: Lemma
+  (requires (raw_data_item_ints_optimal x == true))
+  (ensures (raw_data_item_ints_optimal (cbor_raw_sort x) == true))
+= assert_norm (raw_data_item_ints_optimal == holds_on_raw_data_item raw_data_item_ints_optimal_elem);
+  holds_on_raw_data_item_eq raw_data_item_ints_optimal_elem x;
+  holds_on_raw_data_item_eq raw_data_item_ints_optimal_elem (cbor_raw_sort x);
+  assert_norm (cbor_raw_sort == raw_data_item_fmap cbor_raw_sort_elem);
+  raw_data_item_fmap_eq cbor_raw_sort_elem x;
+  match x with
+  | Tagged tag v ->
+    cbor_raw_sort_ints_optimal v;
+    cbor_raw_sort_elem_ints_optimal (Tagged tag (cbor_raw_sort v))
+  | Array len v ->
+    list_for_all_map cbor_raw_sort v raw_data_item_ints_optimal raw_data_item_ints_optimal (fun x ->
+      cbor_raw_sort_ints_optimal x
+    )
+  | Map len v ->
+    list_for_all_map (apply_on_pair cbor_raw_sort) v (holds_on_pair raw_data_item_ints_optimal) (holds_on_pair raw_data_item_ints_optimal) (fun x ->
+      cbor_raw_sort_ints_optimal (fst x);
+      cbor_raw_sort_ints_optimal (snd x)
+    );
+    let x' = Map len (List.Tot.map (apply_on_pair cbor_raw_sort) v) in
+    holds_on_raw_data_item_eq raw_data_item_ints_optimal_elem x';
+    cbor_raw_sort_elem_ints_optimal x'
+  | _ -> ()
+
+(*
+let rec cbor_raw_sort_equiv
+  (x: raw_data_item)
+: Lemma
+  (ensures (raw_equiv x (cbor_raw_sort x) == true))
+= raw_equiv_eq x (cbor_raw_sort x);
+  assert_norm (cbor_raw_sort == raw_data_item_fmap cbor_raw_sort_elem);
+  raw_data_item_fmap_eq cbor_raw_sort_elem x;
+  match x with
+  | Tagged tag v ->
+    cbor_raw_sort_equiv v
+  | Array len v ->
+    list_for_all2_map cbor_raw_sort v raw_data_item_ints_optimal raw_data_item_ints_optimal (fun x ->
+      cbor_raw_sort_ints_optimal x
+    )
+  | Map len v ->
+    list_for_all_map (apply_on_pair cbor_raw_sort) v (holds_on_pair raw_data_item_ints_optimal) (holds_on_pair raw_data_item_ints_optimal) (fun x ->
+      cbor_raw_sort_ints_optimal (fst x);
+      cbor_raw_sort_ints_optimal (snd x)
+    );
+    let x' = Map len (List.Tot.map (apply_on_pair cbor_raw_sort) v) in
+    holds_on_raw_data_item_eq raw_data_item_ints_optimal_elem x';
+    cbor_raw_sort_elem_ints_optimal x'
+  | _ -> ()
